WIP

code/ecdsa/Hacl.Impl.ECDSA.MM.Exponent.fst
@@ -1,6 +1,5 @@
 module Hacl.Impl.ECDSA.MM.Exponent
 
-
 open FStar.HyperStack.All
 open FStar.HyperStack
 module ST = FStar.HyperStack.ST
@@ -25,31 +24,22 @@ open Hacl.Spec.EC.Definition
 open Hacl.Spec.ECDSA.Definition
 open Hacl.Impl.MM.Exponent
 
-#reset-options " --z3rlimit 200"
 
+#set-options " --z3rlimit 200 --max_fuel 0 --max_ifuel 0"
 
-let montgomery_ladder_exponent #c r = 
-  push_frame(); 
-    let p = create (size 4) (u64 0) in  
-    upload_one_montg_form #c p; 
-    recall_contents (order_inverse_buffer #P256) (prime_order_inverse_seq #P256);
-    let h = ST.get() in
-    mut_const_immut_disjoint #uint64 #uint8 p (order_inverse_buffer #P256) h;
-    mut_const_immut_disjoint #uint64 #uint8 r (order_inverse_buffer #P256) h;
-    assert (disjoint p (order_inverse_buffer #P256));
-    assert (disjoint r (order_inverse_buffer #P256));
-    _montgomery_ladder_power #c #DSA p r (order_inverse_buffer #P256);
-      lemmaToDomainFromDomain #c #DSA 1;
-    copy r p;
-  pop_frame()  
-
+let montgomery_ladder_exponent #c a r = 
+  recall_contents (order_inverse_buffer #c) (prime_order_inverse_seq #c);
+  montgomery_ladder_power #c #DSA a (order_inverse_buffer #c) r
 
 let fromDomainImpl #c a result = 
+  let h0 = ST.get() in 
   push_frame();
-    let one = create (size 4) (u64 0) in 
+    let len = getCoordinateLenU64 c in 
+    let one = create len (u64 0) in 
     uploadOneImpl #c one;
     montgomery_multiplication_buffer_dsa one a result;
-  pop_frame()   
+    lemmaFromDomain #c #DSA (as_nat c h0 a);
+  pop_frame()
 
 
 val lemma_fromDomain1: #c: curve -> a: nat -> 
@@ -95,41 +85,82 @@ let lemma_fromDomain2 a =
 
 let multPower #c a b result = 
   push_frame();
-    let tempB1 = create (size 4) (u64 0) in 
-    let buffFromDB = create (size 4) (u64 0) in 
+    let len = getCoordinateLenU64 c in 
+    let tempB1 = create len (u64 0) in 
+    let buffFromDB = create len (u64 0) in 
 	let h0 = ST.get() in 
       fromDomainImpl #c a tempB1;
       fromDomainImpl #c b buffFromDB;
+	let h1 = ST.get() in 
       fromDomainImpl #c buffFromDB buffFromDB;
-      montgomery_ladder_exponent #c tempB1;
+	let h2 = ST.get() in 
+      montgomery_ladder_exponent #c tempB1 tempB1;
       montgomery_multiplication_buffer_dsa tempB1 buffFromDB result;
+      	let h3 = ST.get() in 
     pop_frame();
-    
-      let p = pow (fromDomain_ #c #DSA (fromDomain_ #c #DSA (as_nat c h0 a))) (prime_p256_order - 2) % prime_p256_order in 
-      let q = fromDomain_ #c #DSA (fromDomain_ #c #DSA (fromDomain_ #c #DSA (as_nat c h0 b))) in 
-      let r = modp_inv2_prime (pow2 256) prime_p256_order in 
-      lemma_fromDomain1 #c (as_nat c h0 b);
-      lemma_fromDomain2 #c (as_nat c h0 a);
+ 
+  let a = as_nat c h0 a in 
+  let b = as_nat c h0 b in 
+  let order = getOrder #c in 
+  let r = modp_inv2_prime (pow2 (getPower c)) order in  
 
-      lemma_mod_mul_distr_l (pow (as_nat c h0 a) (prime_p256_order - 2) * pow r (prime_p256_order - 2) * pow r (prime_p256_order - 2)) (((as_nat c h0 b) * r * r * r) % prime_p256_order) prime_p256_order;
-      lemma_mod_mul_distr_r (pow (as_nat c h0 a) (prime_p256_order - 2) * pow r (prime_p256_order - 2) * pow r (prime_p256_order - 2)) ((as_nat c h0 b) * r * r * r) prime_p256_order;
+  lemma_exp_not_zero order (pow2 (getPower c) % order) (order - 2);
+  Hacl.Impl.EC.Math.lemma_a_not_zero_b_not_zero_mod_not_zero order (r % order) (r % order);
+  lemma_mod_mul_distr_l r (r % order) order;
+  lemma_mod_mul_distr_r r r order;
 
-      assert_by_tactic (pow (as_nat c h0 a) (prime_p256_order - 2) * pow r (prime_p256_order - 2) * pow r (prime_p256_order - 2) * ((as_nat c h0 b) * r * r * r) == pow (as_nat c h0 a) (prime_p256_order - 2) * (pow r (prime_p256_order - 2) * r) * (pow r (prime_p256_order - 2) * r) * (as_nat c h0 b) * r) canon;
+  calc (==) {
+    pow (r * r) (order - 2) * r * r % order;
+    (==) {assert_by_tactic (pow (r * r) (order - 2) * r * r == (r * r) * pow (r * r) (order - 2)) canon} 
+    (r * r) * pow (r * r) (order - 2) % order; 
+    (==) {lemma_mod_mul_distr_r (r * r) (pow (r * r) (order - 2)) order}
+    (r * r) * (pow (r * r) (order - 2) % order) % order;  
+    (==) {power_distributivity (r * r) (order - 2) order}
+    (r * r) * (pow (r * r % order) (order - 2) % order) % order; 
+    (==) {lemma_pow_mod_n_is_fpow order (r * r % order) (order - 2)}
+    (r * r) * (Spec.ECC.Curves.modp_inv2_prime (r * r) order) % order; 
+    (==) {Hacl.Spec.MontgomeryMultiplication.lemma_mod_inv2_mult_prime order (r * r)}
+    1;};
 
-      pow_plus r (prime_p256_order - 2) 1; 
-      power_one r; 
-      lemma_mod_mul_distr_l (pow (as_nat c h0 a) (prime_p256_order - 2) * (pow r (prime_p256_order - 1)) * (pow r (prime_p256_order - 1)) * (as_nat c h0 b) * r) (pow2 256) prime_p256_order;
-      
-      assert_by_tactic (pow (as_nat c h0 a) (prime_p256_order - 2) * (pow r (prime_p256_order - 1)) * (pow r (prime_p256_order - 1)) * (as_nat c h0 b) * r * pow2 256 == pow (as_nat c h0 a) (prime_p256_order - 2) * (pow r (prime_p256_order - 1)) * (pow r (prime_p256_order - 1)) * (as_nat c h0 b) * (r * pow2 256)) canon;
-      lemma_mod_mul_distr_r (pow (as_nat c h0 a) (prime_p256_order - 2) * (pow r (prime_p256_order - 1)) * (pow r (prime_p256_order - 1)) * (as_nat c h0 b)) (r * pow2 256) prime_p256_order;
 
-      assert_norm ((pow2 256 * modp_inv2_prime (pow2 256) prime_p256_order) % prime_p256_order == 1);
-      assert_by_tactic (pow (as_nat c h0 a) (prime_p256_order - 2) * (pow r (prime_p256_order - 1)) * (pow r (prime_p256_order - 1)) * (as_nat c h0 b) == pow (as_nat c h0 a) (prime_p256_order - 2) * (as_nat c h0 b)  * (pow r (prime_p256_order - 1)) * (pow r (prime_p256_order - 1))) canon;
+  calc (==) {
+    toDomain_ #c #DSA (exponent_spec #c (fromDomain_ #c #DSA (fromDomain_ #c #DSA a)) * fromDomain_ #c #DSA (fromDomain_ #c #DSA (fromDomain_ #c #DSA b)) % order);
+    (==) {} 
+    toDomain_ #c #DSA (pow (fromDomain_ #c #DSA (fromDomain_ #c #DSA a)) (order - 2) % order * fromDomain_ #c #DSA (fromDomain_ #c #DSA (fromDomain_ #c #DSA b)) % order); 
+    (==) {lemmaFromDomain #c #DSA a}
+    toDomain_ #c #DSA (pow (fromDomain_ #c #DSA (a * r % order)) (order - 2) % order * fromDomain_ #c #DSA (fromDomain_ #c #DSA (fromDomain_ #c #DSA b)) % order); 
+    (==) {lemmaFromDomain #c #DSA (a * r % order)}
+    toDomain_ #c #DSA (pow ((a * r % order * r % order)) (order - 2) % order * fromDomain_ #c #DSA (fromDomain_ #c #DSA (fromDomain_ #c #DSA b)) % order); 
+    (==) {lemma_mod_mul_distr_l (a * r) r order}
+    toDomain_ #c #DSA (pow (a * r * r % order) (order - 2) % order * fromDomain_ #c #DSA (fromDomain_ #c #DSA (fromDomain_ #c #DSA b)) % order); 
+    (==) {power_distributivity (a * r * r) (order - 2) order}
+    toDomain_ #c #DSA (pow (a * r * r) (order - 2) % order * fromDomain_ #c #DSA (fromDomain_ #c #DSA (fromDomain_ #c #DSA b)) % order); 
+    (==) {assert_by_tactic (a * r * r == a * (r * r)) canon}
+    toDomain_ #c #DSA (pow (a * (r * r)) (order - 2) % order * fromDomain_ #c #DSA (fromDomain_ #c #DSA (fromDomain_ #c #DSA b)) % order); 
+    (==) {lemmaFromDomain #c #DSA b; lemmaFromDomain #c #DSA (b * r % order)}
+    toDomain_ #c #DSA (pow (a * (r * r)) (order - 2) % order * fromDomain_ #c #DSA ((b * r % order) * r % order) % order); 
+    (==) {power_distributivity_2 a (r * r) (order - 2)}
+    toDomain_ #c #DSA ((pow a (order - 2) * pow (r * r) (order - 2)) % order * fromDomain_ #c #DSA ((b * r % order) * r % order) % order); 
+    (==) {lemma_mod_mul_distr_l (pow a (order - 2) * pow (r * r) (order - 2)) (fromDomain_ #c #DSA ((b * r % order) * r % order)) order}
+    toDomain_ #c #DSA (pow a (order - 2) * pow (r * r) (order - 2) * fromDomain_ #c #DSA ((b * r % order) * r % order) % order); 
+    (==) {lemmaFromDomain #c #DSA ((b * r % order) * r % order)}
+    toDomain_ #c #DSA (pow a (order - 2) * pow (r * r) (order - 2) * ((b * r % order) * r % order * r % order) % order); 
+    (==) {lemma_mod_mul_distr_l (b * r) r order}
+    toDomain_ #c #DSA (pow a (order - 2) * pow (r * r) (order - 2) * (b * r * r % order * r % order) % order); 
+    (==) {lemma_mod_mul_distr_l (b * r * r) r order}
+    toDomain_ #c #DSA (pow a (order - 2) * pow (r * r) (order - 2) * (b * r * r * r % order) % order); 
+    (==) {lemma_mod_mul_distr_r (pow a (order - 2) * pow (r * r) (order - 2)) (b * r * r * r) order}
+    toDomain_ #c #DSA (pow a (order - 2) * pow (r * r) (order - 2) * (b * r * r * r) % order); 
+    (==) {assert_by_tactic (pow a (order - 2) * pow (r * r) (order - 2) * (b * r * r * r) == 
+      (r * (pow a (order - 2) * b * (pow (r * r) (order - 2) * r * r)))) canon}
+    toDomain_ #c #DSA (r * (pow a (order - 2) * b * (pow (r * r) (order - 2) * r * r)) % order); 
+    (==) {lemmaFromDomain #c #DSA ((pow a (order - 2) * b * (pow (r * r) (order - 2) * r * r)))}
+    toDomain_ #c #DSA (fromDomain_ #c #DSA (pow a (order - 2) * b * (pow (r * r) (order - 2) * r * r))); 
+    (==) {lemmaToDomainFromDomainModuloPrime #c #DSA (pow a (order - 2) * b * (pow (r * r) (order - 2) * r * r))}
+    (pow a (order - 2) * b * (pow (r * r) (order - 2) * r * r)) % order; 
+    (==) {lemma_mod_mul_distr_r (pow a (order - 2) * b) (pow (r * r) (order - 2) * r * r) order}
+    (pow a (order - 2) * b * (pow (r * r) (order - 2) * r * r % order)) % order;}
 
-      lemma_mod_mul_distr_r (pow (as_nat c h0 a) (prime_p256_order - 2) * (as_nat c h0 b)  * (pow r (prime_p256_order - 1))) (pow r (prime_p256_order - 1)) prime_p256_order;
-
-      lemma_l_ferm ();
-      lemma_mod_mul_distr_r (pow (as_nat c h0 a) (prime_p256_order - 2) * (as_nat c h0 b)) (pow r (prime_p256_order - 1)) prime_p256_order
 
 
 let multPowerPartial #c s a b result = 
