code/ecdsa/Hacl.Impl.ECDSA.Verification.fst
@@ -179,7 +179,7 @@ let ecdsa_verification_step4 #c bufferU1 bufferU2 r s hash =
     let u2 = sub tempBuffer (size 8) (size 4) in
 
     fromDomainImpl s inverseS;
-    montgomery_ladder_exponent #c inverseS;
+    montgomery_ladder_exponent #c inverseS inverseS;
     multPowerPartial s inverseS hash u1;
     multPowerPartial s inverseS r u2;
   
