code/ecdsa/Hacl.P256.fst
@@ -42,10 +42,11 @@ let ecdsa_sign_p256_sha512 result mLen m privKey k =
 let ecdsa_sign_p256_without_hash result mLen m privKey k = 
   ecdsa_signature P256 NoHash result mLen m privKey k
 
-
+*)
 let ecdsa_verif_p256_sha2 mLen m pubKey r s = 
   ecdsa_verification P256 (Hash SHA2_256) pubKey r s mLen m
 
+(*)
 let ecdsa_verif_p256_sha384 mLen m pubKey r s = 
   ecdsa_verification P256 (Hash SHA2_384) pubKey r s mLen m
 
@@ -76,12 +77,12 @@ let compression_compressed_form b result =
 
 
  *)
-let ecp256dh_i result scalar = Hacl.Impl.P256.DH.ecp256dh_i P256 result scalar
+let ecp256dh_i result scalar = Hacl.Impl.EC.DH.ecp256dh_i P256 result scalar
 
-let ecp384dh_i result scalar = Hacl.Impl.P256.DH.ecp256dh_i P384 result scalar
+let ecp384dh_i result scalar = Hacl.Impl.EC.DH.ecp256dh_i P384 result scalar
 
 
-let ecp256dh_r result pubKey scalar = Hacl.Impl.P256.DH.ecp256dh_r #P256 result pubKey scalar
+let ecp256dh_r result pubKey scalar = Hacl.Impl.EC.DH.ecp256dh_r #P256 result pubKey scalar
 
-let ecp384dh_r result pubKey scalar = Hacl.Impl.P256.DH.ecp256dh_r #P384 result pubKey scalar
+let ecp384dh_r result pubKey scalar = Hacl.Impl.EC.DH.ecp256dh_r #P384 result pubKey scalar
 
